update values from BCD

DenotSem/Values.thy
@@ -2,101 +2,97 @@ theory Values
 imports Main
 begin
 
-datatype val = VNat nat | VFun "entry list" and
-  entry = Entry val val (infix "\<mapsto>" 70)
+datatype val = VNat nat | VFun "(val \<times> val) list" 
 
+abbreviation make_entry :: "val \<Rightarrow> val \<Rightarrow> val" (infix "\<mapsto>" 70) where
+  "v \<mapsto> v' \<equiv> VFun [(v,v')]"
+abbreviation bottom_fun :: "val" ("\<bottom>" 100) where
+  "bottom_fun \<equiv> VFun []"
+  
+type_synonym entry = "val \<times> val" 
 type_synonym func = "entry list"  
   
+fun val_join :: "val \<Rightarrow> val \<Rightarrow> val option" (infix "\<squnion>" 56) where
+  "VNat n1 \<squnion> VNat n2 = (if n1 = n2 then Some (VNat n1) else None)" |
+  vfun_join: "VFun f1 \<squnion> VFun f2 = Some (VFun (f1 @ f2))" |
+  "v1 \<squnion> v2 = None"
+
+  (* Adapted from BCD subtyping (Lambda Calculus with Types 2013), but with nu instead of U *) 
+inductive val_le :: "val \<Rightarrow> val \<Rightarrow> bool" (infix "\<sqsubseteq>" 52) where
+  le_refl[intro!]: "(v::val) \<sqsubseteq> v" |
+  le_trans[trans]: "\<lbrakk> (v1::val) \<sqsubseteq> v2; v2 \<sqsubseteq> v3 \<rbrakk> \<Longrightarrow> v1 \<sqsubseteq> v3" |
+  le_join_left: "v1 \<squnion> v2 = Some v12 \<Longrightarrow> v1 \<sqsubseteq> v12" | (* incl_L *)
+  le_join_right[intro!]: "v1 \<squnion> v2 = Some v12 \<Longrightarrow> v2 \<sqsubseteq> v12" | (* incl_R *)
+  le_left_join[intro!]: "\<lbrakk> v1 \<sqsubseteq> v3; v2 \<sqsubseteq> v3; v1 \<squnion> v2 = Some v12\<rbrakk> \<Longrightarrow> v12 \<sqsubseteq> v3" | (* glb *)
+  le_bot[intro!]: "\<bottom> \<sqsubseteq> v \<mapsto> v'" (* nu *) |
+  le_fun[intro!]: "\<lbrakk> v2 \<sqsubseteq> v1; v1' \<sqsubseteq> v2' \<rbrakk> \<Longrightarrow> v1 \<mapsto> v1' \<sqsubseteq> v2 \<mapsto> v2'" | (* arrow *)
+  le_distr: "\<lbrakk> v1 \<squnion> v2 = Some v12; (v\<mapsto>v1) \<squnion> (v \<mapsto>v2) = Some vv12 \<rbrakk>
+     \<Longrightarrow> v \<mapsto> v12 \<sqsubseteq> vv12" (* arrow intersect *)
+
 inductive consistent :: "val \<Rightarrow> val \<Rightarrow> bool" (infix "~" 52) and
     inconsistent :: "val \<Rightarrow> val \<Rightarrow> bool" (infix "!~" 52) where
   vnat_consis[intro!]: "(VNat n) ~ (VNat n)" |
-  vfun_consis[intro!]: "\<lbrakk> \<forall> v1 v1' v2 v2'. v1 \<mapsto>v1' \<in> set t1 \<and> v2\<mapsto>v2' \<in> set t2 \<longrightarrow>
-                        (v1 ~ v2 \<and> v1' ~ v2') \<or> v1 !~ v2 \<rbrakk> \<Longrightarrow> (VFun t1) ~ (VFun t2)" |
+  vfun_consis[intro!]: "\<lbrakk> \<forall> v1 v1' v2 v2'. v1\<mapsto>v1' \<sqsubseteq> VFun f1 \<and> v2\<mapsto>v2' \<sqsubseteq> VFun f2 \<longrightarrow>
+                        (v1 ~ v2 \<and> v1' ~ v2') \<or> v1 !~ v2 \<rbrakk> \<Longrightarrow> (VFun f1) ~ (VFun f2)" |
   vnat_inconsis[intro!]: "n \<noteq> n' \<Longrightarrow> (VNat n) !~ (VNat n')" |
-  vfun_inconsis[intro!]: "\<lbrakk> v1\<mapsto>v1' \<in> set t1; v2\<mapsto>v2' \<in> set t2; v1 ~ v2; v1' !~ v2' \<rbrakk> 
-                         \<Longrightarrow> (VFun t1) !~ (VFun t2)" |
-  vnat_vfun_inconsis[intro!]: "VNat n !~ VFun t" |
-  vfun_vnat_inconsis[intro!]: "VFun t !~ VNat n"
-  
+  vfun_inconsis[intro!]: "\<lbrakk> v1 \<mapsto> v1' \<sqsubseteq> VFun f1; v2 \<mapsto> v2' \<sqsubseteq> VFun f2; v1 ~ v2; v1' !~ v2' \<rbrakk> 
+                         \<Longrightarrow> (VFun f1) !~ (VFun f2)" |
+  vnat_vfun_inconsis[intro!]: "VNat n !~ VFun f" |
+  vfun_vnat_inconsis[intro!]: "VFun f !~ VNat n"
+
 inductive_cases 
   vnat_consis_inv[elim!]: "VNat n ~ VNat n'" and
-  vfun_consis_inv[elim!]: "VFun t ~ VFun t'" and
+  vfun_consis_inv[elim!]: "VFun f ~ VFun f'" and
   vnat_inconsis_inv[elim!]: "VNat n !~ VNat n'" and
-  vfun_inconsis_inv[elim!]: "VFun t !~ VFun t'" and
-  vnat_vfun_consis_inv[elim!]: "VNat n ~ VFun t" and
-  vfun_vnat_consis_inv[elim!]: "VFun t ~ VNat n"
+  vfun_inconsis_inv[elim!]: "VFun f !~ VFun f'" and
+  vnat_vfun_consis_inv[elim!]: "VNat n ~ VFun f" and
+  vfun_vnat_consis_inv[elim!]: "VFun f ~ VNat n"
   
 inductive consis_env :: "val list \<Rightarrow> val list \<Rightarrow> bool" where
   consis_env_nil[intro!]: "consis_env [] []" |
   consis_env_cons[intro!]: "\<lbrakk> v ~ v'; consis_env \<rho> \<rho>' \<rbrakk> \<Longrightarrow> consis_env (v#\<rho>) (v'#\<rho>')" 
 
 definition is_fun :: "func \<Rightarrow> bool" where
-  "is_fun t \<equiv> (\<forall> v1 v2 v1' v2'. v1\<mapsto>v1' \<in> set t \<and> v2\<mapsto>v2' \<in> set t \<and> v1 ~ v2 \<longrightarrow> v1' ~ v2')"
+  "is_fun f \<equiv> VFun f ~ VFun f"
     
 inductive is_val :: "val \<Rightarrow> bool" where
   vnat_is_val[intro!]: "is_val (VNat n)" |
-  vfun_is_val[intro!]: "\<lbrakk> is_fun t; \<forall> v v'. v\<mapsto>v' \<in> set t \<longrightarrow> is_val v \<and> is_val v' \<rbrakk>
-                        \<Longrightarrow> is_val (VFun t)"
+  vfun_is_val[intro!]: "\<lbrakk> is_fun f; \<forall> v v'. (v,v') \<in> set f \<longrightarrow> is_val v \<and> is_val v' \<rbrakk>
+                        \<Longrightarrow> is_val (VFun f)"
 inductive_cases
-  vfun_is_val_inv[elim!]: "is_val (VFun t)"
+  vfun_is_val_inv[elim!]: "is_val (VFun f)"
 
 definition val_env :: "val list \<Rightarrow> bool" where
   "val_env \<rho> \<equiv> \<forall>k. k < length \<rho> \<longrightarrow> is_val (\<rho>!k)"
-  
-fun val_join :: "val \<Rightarrow> val \<Rightarrow> val" (infix "\<squnion>" 56) where
-  "VNat n1 \<squnion> VNat n2 = (if n1 = n2 then VNat n1 else undefined)" |
-  vfun_join: "VFun f1 \<squnion> VFun f2 = (VFun (f1 @ f2))" |
-  "v1 \<squnion> v2 = undefined"
-  
-fun env_join :: "val list \<Rightarrow> val list \<Rightarrow> val list" (infix "\<squnion>" 56) where
-  "env_join [] [] = []" |
-  "env_join (v#\<rho>) (v'#\<rho>') = (v \<squnion> v')#(env_join \<rho> \<rho>')" |
-  "env_join \<rho> \<rho>' = undefined" 
 
-inductive val_le :: "val \<Rightarrow> val \<Rightarrow> bool" (infix "\<sqsubseteq>" 52) and
-    entry_le :: "entry \<Rightarrow> entry \<Rightarrow> bool" (infix "\<sqsubseteq>" 52) and
-    fun_le :: "func \<Rightarrow> func \<Rightarrow> bool" (infix "\<sqsubseteq>" 52) and
-    fun_in :: "entry \<Rightarrow> func \<Rightarrow> bool" ("_ in _" [56,56] 55)
-    where
-  vnat_le[intro!]: "(VNat n) \<sqsubseteq> (VNat n)" |
-  vfun_le[intro!]: "t1 \<sqsubseteq> t2 \<Longrightarrow> (VFun t1) \<sqsubseteq> (VFun t2)" |
-  entry_le[intro!]: "\<lbrakk> v2 \<sqsubseteq> v1; v1' \<sqsubseteq> v2'\<rbrakk> \<Longrightarrow> (v1\<mapsto>v1') \<sqsubseteq> (v2\<mapsto>v2')" |
-  empty_le[intro!]: "[] \<sqsubseteq> t2" |
-  ins_le[intro!]: "\<lbrakk> p in t2; t1 \<sqsubseteq> t2 \<rbrakk> \<Longrightarrow>  p#t1 \<sqsubseteq> t2" |
-  fun_in_ax[intro!]: "\<lbrakk> p \<in> set t \<rbrakk> \<Longrightarrow> p in t" |
-  fun_in_sub: "\<lbrakk> p1 in t; p1 \<sqsubseteq> p2 \<rbrakk> \<Longrightarrow> p2 in t" 
-(*
-  fun_in_union: "\<lbrakk> (v1,v1') in t; (v2,v2') in t; v \<sqsubseteq> v1 \<squnion> v2; v1' \<squnion> v2' \<sqsubseteq> v' \<rbrakk>
-                   \<Longrightarrow> (v,v') in t"
-*)
-  
+fun env_join :: "val list \<Rightarrow> val list \<Rightarrow> (val list) option" (infix "\<squnion>" 56) where
+  "env_join [] [] = Some []" |
+  "env_join (v#\<rho>) (v'#\<rho>') =
+     (case (v \<squnion> v') of
+        None \<Rightarrow> None
+      | Some v'' \<Rightarrow> 
+        (case env_join \<rho> \<rho>' of
+          None \<Rightarrow> None
+        | Some \<rho>'' \<Rightarrow> Some (v''#\<rho>'')))" |
+  "env_join \<rho> \<rho>' = None" 
+ 
 definition env_le :: "val list \<Rightarrow> val list \<Rightarrow> bool" (infix "\<sqsubseteq>" 52) where 
   "(\<rho>::val list) \<sqsubseteq> \<rho>' \<equiv> length \<rho> = length \<rho>' \<and> (\<forall> k. k < length \<rho>  \<longrightarrow> \<rho>!k \<sqsubseteq> \<rho>'!k)" 
 
-inductive_cases 
-  le_fun_fun_inv[elim!]: "VFun t1 \<sqsubseteq> VFun t2" and
-  le_fun_nat_inv[elim!]: "VFun t2 \<sqsubseteq> VNat x1" and
-  le_any_nat_inv[elim!]: "v \<sqsubseteq> VNat n" and
-  le_nat_any_inv[elim!]: "VNat n \<sqsubseteq> v" and
-  le_fun_any_inv[elim!]: "VFun t \<sqsubseteq> v" and
-  le_any_fun_inv[elim!]: "v \<sqsubseteq> VFun t" and
-  le_cons_fun_inv[elim!]: "((p::entry)#t1) \<sqsubseteq> t2"
-  
-section "Joins and Meets"
-  
-abbreviation val_lub :: "val \<Rightarrow> val \<Rightarrow> val \<Rightarrow> bool" where
-  "val_lub v v1 v2 \<equiv> v1 \<sqsubseteq> v \<and> v2 \<sqsubseteq> v \<and> (\<forall> v'. v1 \<sqsubseteq> v' \<and> v2 \<sqsubseteq> v' \<longrightarrow> v \<sqsubseteq> v')"
-
-abbreviation val_glb :: "val \<Rightarrow> val \<Rightarrow> val \<Rightarrow> bool" where
-  "val_glb v v1 v2 \<equiv> v \<sqsubseteq> v1 \<and> v \<sqsubseteq> v2 \<and> (\<forall> v'. v' \<sqsubseteq> v1 \<and> v' \<sqsubseteq> v2 \<longrightarrow> v' \<sqsubseteq> v)"
-
 section "Size of Values (for induction)"
   
-primrec vsize :: "val \<Rightarrow> nat" and esize :: "entry \<Rightarrow> nat" and fsize :: "func \<Rightarrow> nat" where
+function vsize :: "val \<Rightarrow> nat" and fsize :: "func \<Rightarrow> nat" where
 "vsize (VNat n) = 1" |
 "vsize (VFun t) = 1 + fsize t" |
-"esize (v\<mapsto>v') = 1+ vsize v + vsize v'" |
 "fsize [] = 0" |
-"fsize (e#t) = 1+ esize e + fsize t"
+"fsize ((v,v')#t) = 1 + vsize v + vsize v' + fsize t"
+  by pat_completeness auto
+termination vsize by size_change
+      
+lemma "(v1 ~ v2 \<longrightarrow> (\<exists> v3. v1 \<squnion> v2 = Some v3))
+      \<and> (v1 !~ v2 \<longrightarrow> True)"
+  by (induction rule: consistent_inconsistent.induct) auto
 
+    
+  
 end
